eve/Src/framework/eve_proofs/writer/ep_constant_writer.e
@@ -31,7 +31,7 @@ feature -- Basic operations
 			l_type := type_mapper.boogie_type_for_type (a_feature.type)
 
 			put_comment_line ("Functional represenation of constant")
-			put_line ("function " + l_functional_name + "(heap: [ref, <x>name]x, current: ref) returns (" + l_type + ");")
+			put_line ("function " + l_functional_name + "(heap: HeapType, current: ref) returns (" + l_type + ");")
 			put_new_line
 
 			if l_constant.value.is_boolean then
@@ -53,7 +53,7 @@ feature -- Basic operations
 				put_comment_line ("Unsupported type, no axiom generated")
 			else
 				put_comment_line ("Axiomatic mapping of function to constant value")
-				put_line ("axiom (forall heap: [ref, <x>name]x, current: ref ::")
+				put_line ("axiom (forall heap: HeapType, current: ref ::")
 				put_line ("            { " + l_functional_name + "(heap, current) } // Trigger");
 				put_line ("        IsHeap(heap) ==> (" + l_functional_name + "(heap, current) == " + l_value + "));")
 				put_new_line
